#
# Vocabulary to define vocabularies with properties that point to different members of an RDF list.
#
# You can define properties to point to any member, plus the first and the last.
#
# Author: Tobias KÃ¤fer
#

#
# Example for talking about children and descendants of a node in a tree:
#
## The child relation:
# ex:hasChild
#   ldf:accompanying ex:hasChildren ;
#   rdfs:subPropertyOf ex:hasDescendant .
#
## The descendant relation:
# ex:hasDescendant
#   a owl:TransitiveProperty .
#
#
## The left-most child and descendant:
# ex:hasLeftMostChild
#   :isLast ex:hasChild ;
#   rdfs:subPropertyOf ex:hasLeftMostDescendant .
#
# ex:hasLeftMostDescendant
#   a owl:TransitiveProperty .
# 
#
## The right-most child and descendant: 
# ex:hasRightMostChild
#   :isLast ex:hasChild ;
#   rdfs:subPropertyOf ex:hasRightMostDescendant .
# 
# ex:hasRightMostDescendant
#   a owl:TransitiveProperty .
#

@base <http://purl.org/list/vocab> .

@prefix : <#> .
@prefix rdf: <http://www.w3.org/1999/02/22-rdf-syntax-ns#> .
@prefix rdfs: <http://www.w3.org/2000/01/rdf-schema#> .
@prefix owl: <http://www.w3.org/2002/07/owl#> .

<> rdfs:seeAlso <semantics> .

#
# Classes
#

:ListMembershipProperty a rdfs:Class ;
  rdfs:label "List Membership Property" ;
  rdfs:comment "The class of properties that point from a thing to entries in a list attached to the thing." ;
  rdfs:isDefinedBy <semantics> , <> .

:FirstMemberProperty a rdfs:Class ;
  rdfs:label "First List Item Membership Property" ;
  rdfs:comment "The class of properties that point from a thing to the first entry in a list attached to the thing." ;
  rdfs:isDefinedBy <semantics> , <> .

:LastMemberProperty a rdfs:Class ;
  rdfs:label "Last List Item Membership Property" ;
  rdfs:comment "The class of properties that point from a thing to the last entry in a list attached to the thing." ;
  rdfs:isDefinedBy <semantics> , <> .

#
# Properties
#

:accompanying
  a rdf:Property ;
  rdfs:label "accompanying" ;
  rdfs:comment "States that a list membership property accompanies a property." ;
  rdfs:domain :ListMembershipProperty ;
  rdfs:range rdf:Property ;
  rdfs:isDefinedBy <semantics> , <> .

:isLast
  a rdf:Property ;
  rdfs:label "is last" ;
  rdfs:comment "Corresponds to list membership property pointing to the last item in the list." ;
  rdfs:subPropertyOf rdfs:subPropertyOf ;
  rdfs:domain :LastMemberProperty ;
  rdfs:range :ListMembershipProperty ;
  rdfs:isDefinedBy <semantics> , <> .

:isFirst
  a rdf:Property ;
  rdfs:label "is first" ;
  rdfs:comment "Corresponds to list membership property pointing to the First item in the list." ;
  rdfs:subPropertyOf rdfs:subPropertyOf ;
  rdfs:domain :FirstMemberProperty ;
  rdfs:range :ListMembershipProperty ;
  rdfs:isDefinedBy <semantics> , <> .

:transitiveRest
  a rdf:Property , owl:TransitiveProperty ;
  rdfs:label "rest, transitively" ;
  rdfs:comment "A transitive version for the rest property from the rdf vocabulary." ;
  rdfs:seeAlso rdf:rest ;
  rdfs:isDefinedBy <> .
rdf:rest rdfs:subPropertyOf :transitiveRest .

:equalsOrTransitiveRest a rdf:Property .
:transitiveRest rdfs:subPropertyOf :equalsOrTransitiveRest .

